LiveVerif/src/LiveVerifExamples/Tests/split_conclusion.v
@@ -1,0 +1,131 @@
+(* -*- eval: (load-file "../../LiveVerif/live_verif_setup.el"); -*- *)
+Require Import LiveVerif.LiveVerifLib.
+
+(* Usually, we keep all adjacent memory in the same sep clause, so when canceling,
+   we only need to check if a clause in the hyps is a superrange of the clause
+   in the conclusion to be cancelled.
+   But in tailrec while lemmas, we get a
+   "post-with-small-ghostvars implies post-with-bigger-ghostvars" goal
+   and the post-with-small-ghostvars typically has a bigger frame (containing some
+   deliberately forgotten memory), which might be adjacent to some non-framed
+   memory, but did not get merged together, so during the cancellation to prove
+   post-with-bigger-ghostvars, we would need to merge in the hyps, or to split
+   in the conclusion, and we chose to split in the conclusion (because currently,
+   we never do a search for anything mergeable in the hyps, we only merge back
+   stuff that was split before a function call). *)
+
+Load LiveVerif.
+
+(*
+
+
+
+Example: We're trying to cancel in order 1-2-3, upper line is hyps,
+lower line is conclusion.
+Note that conclusion clause #1 is not a subrange of any hyp clause,
+and no hyp clause is a subrange of a conclusion clause.
+But there is a hyp clause whose beginning points into the middle of
+conclusion clause 1, so we split the conclusion there, and then continue
+as usual by splitting hyps that are a superrange of a conclusion clause.
+
+|--------|-------------|
+|--3--|----1--|---2----|
+
+|--------|-------------|
+|--3--|1a|-1b-|---2----|
+
+|-----|xx|-------------|
+|--3--|xx|-1b-|---2----|
+
+
+Alternative (would require flexible cancellation order):
+
+|--------|-------------|
+|--3--|----1--|---2----|
+
+delay cancellation of 1
+
+|--------|----|xxxxxxxx|
+|--3--|----1--|xxxxxxxx|
+
+|xxxxx|--|----|xxxxxxxx|
+|xxxxx|----1--|xxxxxxxx|
+
+now we have a hyp clause that's a subrange of the conclusion clause, so split:
+
+|xxxxx|--|----|xxxxxxxx|
+|xxxxx|1a|-1b-|xxxxxxxx|
+
+
+Every boundary at which we might need to split the conclusion is both the beginning
+and the end of a range appearing in the hyps, so it's sufficient to only consider
+range beginnings in the hyps. *)
+
+#[export] Instance spec_of_test0: fnspec :=                                      .**/
+
+void test0(uintptr_t p1, uintptr_t p2, uintptr_t n1, uintptr_t n2, uintptr_t p3) /**#
+  ghost_args := (R: mem -> Prop) (vs1 vs2: list Z);
+  requires t m := <{ * array (uint 32) \[n1] vs1 p1
+                     * array (uint 32) \[n2] vs2 p2
+                     * R }> m;
+  ensures t' m' := exists vs, t' = t /\
+            <{ * array (uint 32) (\[n1] + \[n2]) vs p3
+               * R }> m' #**/                                              /**.
+Derive test0 SuchThat (fun_correct! test0) As test0_ok.                         .**/
+{                                                                          /**. .**/
+}                                                                          /**.
+  test_error Error:("Exactly one of the following claims should hold:"
+          [| subrange p3 ((\[n1] + \[n2]) * 4) p1 (\[n1] * 4);
+             inrange p1 p3 ((\[n1] + \[n2]) * 4);
+             subrange p3 ((\[n1] + \[n2]) * 4) p2 (\[n2] * 4);
+             inrange p2 p3 ((\[n1] + \[n2]) * 4)|]).
+Abort.
+
+#[export] Instance spec_of_test: fnspec :=                                      .**/
+
+void test(uintptr_t p1, uintptr_t p2, uintptr_t n1, uintptr_t n2) /**#
+  ghost_args := (R: mem -> Prop) (vs1 vs2: list Z);
+  requires t m := p1 ^+ /[4] ^* n1 = p2 /\ 4 * \[n1] < 2 ^ 32 /\
+                  <{ * array (uint 32) \[n1] vs1 p1
+                     * array (uint 32) \[n2] vs2 p2
+                     * R }> m;
+  ensures t' m' := exists vs, t' = t /\
+            <{ * array (uint 32) (\[n1] + \[n2]) vs p1
+               * R }> m' #**/                                              /**.
+Derive test SuchThat (fun_correct! test) As test_ok.                            .**/
+{                                                                          /**. .**/
+}                                                                          /**.
+  lazymatch goal with
+  | |- split_concl_at ?s ?g =>
+      change g;
+      lazymatch g with
+      | canceling (cons ?P ?Ps) ?om ?Rest =>
+          lazymatch P with
+          | array ?elem ?size ?vs ?start =>
+              eapply cancel_rew_head;
+              [ eapply (split_array_at_bw _ s);
+                [ reflexivity | word_lia_hook_for_split_merge ]
+              | ]
+          end
+      end
+  end.
+
+  step. step. step. step. step. step. step. step.
+
+  step. step. step. step.
+  (* TODO in the goal
+
+  impl1 (array (uint 32) \[n2] vs2 p2)
+        (array (uint 32) (\[n1] + \[n2] - \[p2 ^- p1] / 4) ?vs2 p2)
+
+   careful_reflexivity_step does not dare to instantiate ?vs2.
+   On the other hand, in HeapletwiseHyps, hyp_clause_matches_goal_clause does,
+   and that's why this problem hasn't appeared up to now. *)
+  {
+    replace (\[n1] + \[n2] - \[p2 ^- p1] / 4) with \[n2].
+    1: reflexivity.
+    word_lia_hook_for_split_merge.
+  }
+Abort.
+
+End LiveVerif. Comments .**/ //.
